# The Function Monad

## A Refresher on Monads

Via the `Box` type, we originally learned what a `Monad` even is. To refresh our memory, a data type can be called a `Monad` if it can implement a law-abiding instance for the `Monad` type class. We then used the `Box` type to introduce "do notation," which desugars into nested `bind`/`>>=` calls.

We later showed that using other monadic types like `Maybe`, `Either`, and `List` led to different control flows. `Maybe` led to a nested if-then-else statement. `Either` was similar but returned something when an error occurred. `List` produced a nested `for` loop.

However, we never stopped to consider the data type, `Function`. When we re-examine the `Function` data type, we'll see that it's naturally a `Monad`.

## Reviewing `Function` as a Data Type

Putting it into syntax, `Function` is defined like this:
```purescript
data Function a b = -- implementation

infix ? Function as ->

-- Thus, when we write this:
intToString :: Int -> String
intToString _ = "a string"

-- It desguars to this:
intToString :: Function Int String
intToString _ = "a string"
```

## Implementing the `Monad` Type Class Hierarchy's Functions

Let's start small by not implementing instances for these type classes. Rather, we'll explore how we'd write the actual implementations for their functions.

For now, take my word for it that these implementations satisfy the laws of their respective type classes.

### Functor

#### Initial Problems

Let's look at `Functor`'s `map` function. It's type signature looks like this.
```purescript
map :: forall a b. (a -> b) -> f a -> f b
```

This creates the first problem: `Functor` expects a higher-kinded type, `f`, that only takes one type. For example, `Box a` only takes one type. However, `Function a b` takes two types. So, how can this be resolved? We must assume that `Function a b` already has its first type. For example...
```purescript
data Function a b = -- implementation

noTypesDefined :: forall a b. Function a   b
noTypesDefined = -- implementation

oneTypeDefined :: forall   b. Function Int b
oneTypeDefined = -- implementation

allTypesDefined ::            Function Int Int
allTypesDefined = -- implementation
```
To make `Function` higher-kinded by only one type, and not two, we should use something like `oneTypeDefined` above.

#### Implementing `map`

Getting back to the problem at hand, here's the type signature for Function's `map` implementation with very helpful names:
```purescript
map :: forall input originalOutput newOutput.
      (originalOutput -> newOutput) ->
      Function input originalOutput -> Function input newOutput
```
It should seem pretty obvious how this gets implemented. Let's walk through this slowly.

1. `map` returns a new function whose input is `input`. So, let's use an inline function to do that:
```purescript
map :: forall input originalOutput newOutput.
      (originalOutput -> newOutput) ->
      Function input originalOutput -> Function input newOutput
map originalToNew f = (\input -> {- remaining body of function -} )
```

2. Since `f` is the only function that can "receive" a value of type, `input`, we have to pass that value into `f`. `f` will produce `originalOutput`, so let's store that in a let binding:
```purescript
map :: forall input originalOutput newOutput.
      (originalOutput -> newOutput) ->
      Function input originalOutput -> Function input newOutput
map originalToNew f = (\input ->
  let originalOutput = f argument
  in {- remaining body of function -} )
```

3. Since `originalTonew` is the only function that can "receive" a value of type, `originalOutput`, we have to pass the value outputted by `f` into that function. `originalTonew` produces a value of the type, `newOutput`, which gives us the return value of our created function:
```purescript
map :: forall input originalOutput newOutput.
      (originalOutput -> newOutput) ->
      Function input originalOutput -> Function input newOutput
map originalToNew f = (\input ->
  let originalOutput = f argument
  in originalToNew originalOutput )
```

As we can see, the types guided us on how to implement this function. If we look at this closer, we can see that it's just function composition.
```purescript
map :: forall input originalOutput newOutput.
      (originalOutput -> newOutput) ->
      Function input originalOutput -> Function input newOutput
map originalToNew f = (\input -> originalOutput $ f input)
-- or
map originalToNew f = (originalOutput <<< f)
-- or even
map = (<<<)
```

#### Takeaways

Our first example taught us two things:
- we have to create a new function by using lambda syntax: `\argument -> body`
- we have to assume that `Function` already has its first type (the input) and that the `a` and `b` arguments refer to its second type (the output).

### Apply

#### Initial Problems

Let's now look at `Apply`'s `apply` function. It's type signature looks like this.
```purescript
apply :: forall a b. f (a -> b) -> f a -> f b
```

Again, let's take this slowly. Notice first the first argument, what should the full type signature of `f (a -> b)` be if `f` is `Function`? Since the `f` has to be the same for both situations, then `f` has to be `Function input`. In other words, the first argument is a function that returns another function:
```purescript
apply :: forall input originalOutput newOutput.
         Function input (originalOutput -> newOutput) ->
         Function input  originalOutput ->
         Function input newOutput
```

#### Implementing `apply`

Let's see how to implement this function.

1. Since `apply` returns a new function, let's start creating one using lambda syntax:
```purescript
apply :: forall input originalOutput newOutput.
         Function input (originalOutput -> newOutput) ->
         Function input  originalOutput ->
         Function input newOutput
apply functionInFunction f = (\input -> {- body of function -})
```

2. At this point, both `f` and `functionInFunction` can receive an value of type, `input`. For right now, let's do what we did last time and only pass it into `f`. We'll store the output in a let binding:
```purescript
apply :: forall input originalOutput newOutput.
         Function input (originalOutput -> newOutput) ->
         Function input  originalOutput ->
         Function input newOutput
apply functionInFunction f = (\input ->
  let originalOutput = f input
  in {- body of function -})
```

3. At this point, the only way to get map `originalOutput` into `newOutput` is to pass it into the function that's hidden in `functionInFunction`. How do we get that out? We can pass `input` into that function. Again, we'll store that output in a let binding:
```purescript
apply :: forall input originalOutput newOutput.
         Function input (originalOutput -> newOutput) ->
         Function input  originalOutput ->
         Function input newOutput
apply functionInFunction f = (\input ->
  let
    originalOutput = f input
    originalToNew = functionInFunction input
  in {- body of function -})
```

4. We now have all the pieces we need to return `newOutput`. Let's pass `originalOutput` into `originalTonew`:
```purescript
apply :: forall input originalOutput newOutput.
         Function input (originalOutput -> newOutput) ->
         Function input  originalOutput ->
         Function input newOutput
apply functionInFunction f = (\input ->
  let
    originalOutput = f input
    originalToNew = functionInFunction input
  in originalToNew originalOutput)
```

Great! Can we clean it up now?
```purescript
apply :: forall input originalOutput newOutput.
         Function input (originalOutput -> newOutput) ->
         Function input  originalOutput ->
         Function input newOutput
apply functionInFunction f = (\input -> (functionInFunction input) (f input))
```

#### Takeaways

Our second example taught us the following:
- to get all the pieces necessary to implement a type class' function, we sometimes need to pass the input value into multiple functions.

### Applicative

Let's now look at `Applicative`'s `pure` function. It's type signature looks like this.
```purescript
apply :: forall a. a -> f a
```

Converting `f` into `Function input`, we get this type signature:
```purescript
apply :: forall input output. output -> Function input output
```

Let's see how to implement it.

1. Since `apply` returns a new function, let's start creating one using lambda syntax:
```purescript
apply :: forall input output. output -> Function input output
apply value = (\input -> {- body of function -})
```

2. Since the function must return `value` as its output, let's ignore the argument and just return that value.
```purescript
apply :: forall input output. output -> Function input output
apply value = (\input -> value)
```

Let's clean this one up:
```purescript
apply :: forall input output. output -> Function input output
apply value = (\_ -> value)
```

### Bind

#### Implementing `bind`

Let's now look at `Bind`'s `bind` function. It's type signature looks like this.
```purescript
bind :: forall a b. (a -> m b) -> m a -> m b
```

Converting `m` into `Function input`, we get this type signature:
```purescript
bind :: forall input originalOutput newOutput.
        (originalOutput -> Function input newOutput) ->
        Function input originalOutput ->
        Function input newOutput
```

Let's see how to implement it.

1. Since `bind` returns a new function, let's start creating one using lambda syntax:
```purescript
bind :: forall input originalOutput newOutput.
        (originalOutput -> Function input newOutput) ->
        Function input originalOutput ->
        Function input newOutput
bind originalToFunction f = (\input -> {- body of function -})
```

2. Since `f` is the only function that can "receive" the `input` value, let's pass it into `f` and store the output:
```purescript
bind :: forall input originalOutput newOutput.
        (originalOutput -> Function input newOutput) ->
        Function input originalOutput ->
        Function input newOutput
bind originalToFunction f = (\input ->
  let originalOutput = f input
  in {- body of function -})
```

3. Since `originalToFunction` can "receive" the `originalOutput` value, let's pass that into `originalToFunction` and store its result in a let binding:
```purescript
bind :: forall input originalOutput newOutput.
        (originalOutput -> Function input newOutput) ->
        Function input originalOutput ->
        Function input newOutput
bind originalToFunction f = (\input ->
  let
    originalOutput = f input
    inputToNewOutput = originalToFunction originalOutput
  in {- body of function -})
```

4. Since `inputToNewOutput` is the only function that can produce the `newOutput` value, let's pass `input` into it to get that value:
```purescript
bind :: forall input originalOutput newOutput.
        (originalOutput -> Function input newOutput) ->
        Function input originalOutput ->
        Function input newOutput
bind originalToFunction f = (\input ->
  let
    originalOutput = f input
    inputToNewOutput = originalToFunction originalOutput
  in inputToNewOutput input)
```

Let's now clean it up. First we'll get rid of that `inputToNewOutput` binding:
```purescript
bind :: forall input originalOutput newOutput.
        (originalOutput -> Function input newOutput) ->
        Function input originalOutput ->
        Function input newOutput
bind originalToFunction f = (\input ->
  let
    originalOutput = f input
  in (originalToFunction originalOutput) input)
```

Second, we'll get rid of that `originalOutput` binding:
```purescript
bind :: forall input originalOutput newOutput.
        (originalOutput -> Function input newOutput) ->
        Function input originalOutput ->
        Function input newOutput
bind originalToFunction f = (\input -> (originalToFunction (f input)) input)
```

As can be seen, this example was a slightly more complicated version of `apply` in that we needed to pass `input` to multiple functions.

## Summary of Our Takeaways

- `map` example:
    - we have to create a new function by using lambda syntax: `\argument -> body`
    - we have to assume that `Function` already has its first type (the input) and that the `a`/`originalOutput` and `b`/`newOutput` arguments refer to its second type (the output).
- `apply`/`bind` example:
    - to get all the pieces necessary to return the `b`/`newOutput` value, we sometimes need to pass the `input` value into multiple functions.
